ainvs+access+infoflow+dpolicy: interpret XN as Read on AARCH64
Introduce ptable_exec to use in do_user_op_if. This makes the execute
right available. All architectures have some form of it, but how it is
handled and whether it may imply Read authority or not differs.

Use the new interface in AARCH64 where XN implies Read authority even
for pages without read permission on the PTE. This forces the infoflow
proof to show that the XN fix from the previous commit is sufficient.

Signed-off-by: Gerwin Klein <gerwin.klein@proofcraft.systems>

proof/access-control/ARM/ArchAccess.thy
@@ -12,31 +12,37 @@ context Arch begin arch_global_naming
 
 subsection \<open>Arch-specific transformation of caps into authorities\<close>
 
-definition vspace_cap_rights_to_auth :: "cap_rights \<Rightarrow> auth set" where
-  "vspace_cap_rights_to_auth r \<equiv>
+\<comment> \<open>Execute does not confer Read authority on this architecture and is ignored.\<close>
+definition vspace_cap_rights_to_auth :: "cap_rights \<Rightarrow> bool \<Rightarrow> auth set" where
+  "vspace_cap_rights_to_auth r exec \<equiv>
      (if AllowWrite \<in> r then {Write} else {})
    \<union> (if AllowRead \<in> r then {Read} else {})"
 
 definition arch_cap_auth_conferred where
   "arch_cap_auth_conferred arch_cap \<equiv>
-     (if is_page_cap arch_cap then vspace_cap_rights_to_auth (acap_rights arch_cap) else {Control})"
+     (if is_page_cap arch_cap then vspace_cap_rights_to_auth (acap_rights arch_cap) False
+      else {Control})"
 
 subsection \<open>Generating a policy from the current ASID distribution\<close>
 
 definition pte_ref where
   "pte_ref pte \<equiv> case pte of
      SmallPagePTE addr atts rights
-       \<Rightarrow> Some (ptrFromPAddr addr, pageBitsForSize ARMSmallPage, vspace_cap_rights_to_auth rights)
+       \<Rightarrow> Some (ptrFromPAddr addr, pageBitsForSize ARMSmallPage,
+                vspace_cap_rights_to_auth rights False)
    | LargePagePTE addr atts rights
-       \<Rightarrow> Some (ptrFromPAddr addr, pageBitsForSize ARMLargePage, vspace_cap_rights_to_auth rights)
+       \<Rightarrow> Some (ptrFromPAddr addr, pageBitsForSize ARMLargePage,
+                vspace_cap_rights_to_auth rights False)
    | _ \<Rightarrow> None"
 
 definition pde_ref2 where
   "pde_ref2 pde \<equiv> case pde of
      SectionPDE addr atts domain rights
-       \<Rightarrow> Some (ptrFromPAddr addr, pageBitsForSize ARMSection, vspace_cap_rights_to_auth rights)
+       \<Rightarrow> Some (ptrFromPAddr addr, pageBitsForSize ARMSection,
+                vspace_cap_rights_to_auth rights False)
    | SuperSectionPDE addr atts rights
-       \<Rightarrow> Some (ptrFromPAddr addr, pageBitsForSize ARMSuperSection, vspace_cap_rights_to_auth rights)
+       \<Rightarrow> Some (ptrFromPAddr addr, pageBitsForSize ARMSuperSection,
+                vspace_cap_rights_to_auth rights False)
    | PageTablePDE addr atts domain
        \<comment> \<open>The 0 is a hack, saying that we own only addr, although 12 would also be OK\<close>
        \<Rightarrow> Some (ptrFromPAddr addr, 0, {Control})
