proof/access-control/RISCV64/ArchAccess.thy
@@ -12,14 +12,16 @@ context Arch begin arch_global_naming
 
 subsection \<open>Arch-specific transformation of caps into authorities\<close>
 
-definition vspace_cap_rights_to_auth :: "cap_rights \<Rightarrow> auth set" where
-  "vspace_cap_rights_to_auth r \<equiv>
+\<comment> \<open>Execute does not confer Read authority on this architecture and is ignored.\<close>
+definition vspace_cap_rights_to_auth :: "cap_rights \<Rightarrow> bool \<Rightarrow> auth set" where
+  "vspace_cap_rights_to_auth r exec \<equiv>
      (if AllowWrite \<in> r then {Write} else {})
    \<union> (if AllowRead \<in> r then {Read} else {})"
 
 definition arch_cap_auth_conferred where
   "arch_cap_auth_conferred arch_cap \<equiv>
-     (if is_FrameCap arch_cap then vspace_cap_rights_to_auth (acap_rights arch_cap) else {Control})"
+     (if is_FrameCap arch_cap then vspace_cap_rights_to_auth (acap_rights arch_cap) False
+      else {Control})"
 
 subsection \<open>Generating a policy from the current ASID distribution\<close>
 
@@ -28,7 +30,7 @@ definition pte_ref2 where
      PagePTE ppn atts rights
        \<Rightarrow> Some (ptrFromPAddr (addr_from_ppn ppn),
                 pageBitsForSize (vmpage_size_of_level level),
-                vspace_cap_rights_to_auth rights)
+                vspace_cap_rights_to_auth rights False)
    | PageTablePTE ppn atts
        \<Rightarrow> Some (ptrFromPAddr (addr_from_ppn ppn), 0, {Control})
    | _ \<Rightarrow> None"
